<?xml version="1.0" encoding="UTF-8"?>
<!-- $Author: MarkusDoering $ -->

<rdf:RDF xmlns:rdf="http://www.w3.org/1999/02/22-rdf-syntax-ns#"
   xmlns:rdfs="http://www.w3.org/2000/01/rdf-schema#" xmlns:owl="http://www.w3.org/2002/07/owl#"
   xmlns:dc="http://purl.org/dc/elements/1.1/" xmlns:dcterms="http://purl.org/dc/terms/"
   xmlns:tbase="http://rs.tdwg.org/ontology/Base#" xmlns:tcore="http://rs.tdwg.org/ontology/Core#"
   xmlns:tcom="http://rs.tdwg.org/ontology/voc/Common#"
   xmlns:tor="http://rs.tdwg.org/ontology/voc/OccurrenceRecord#"
   xmlns="http://rs.tdwg.org/ontology/voc/OccurrenceRecord#"
   xml:base="http://rs.tdwg.org/ontology/voc/OccurrenceRecord">

   <owl:Ontology rdf:about="http://rs.tdwg.org/ontology/voc/OccurrenceRecord">
      <dc:title>TDWG OccurrenceRecord LSID Ontology</dc:title>
      <dc:creator>Roger Hyam</dc:creator>
      <dc:publisher>TDWG Biodiversity Information Standards</dc:publisher>
      <dcterms:issued>2006-12-06</dcterms:issued>
      <dcterms:modified>2015-07-01</dcterms:modified>
      <dc:description>Ontology describing the metadata returned for LSIDs that are used taxon
         occurrence records. </dc:description>
      <owl:versionInfo>0.3</owl:versionInfo>
      <owl:deprecated rdf:datatype="http://www.w3.org/2001/XMLSchema#boolean">true</owl:deprecated>
      <rdfs:comment>This ontology is no longer under development and is no longer recommended for use.  See https://github.com/tdwg/ontology for information about recommended replacements.</rdfs:comment>
      <rdfs:seeAlso rdf:resource="https://raw.githubusercontent.com/tdwg/ontology/master/replacements.rdf"/>

      <rdfs:comment rdf:parseType="Literal"> *** This vocabulary has been superseded by the
         TaxonOccurrence vocabulary (http://rs.tdwg.org/ontology/voc/TaxonOccurrence) Read more
         about this on the associated wiki page.**** This ontology is designed to represent records
         of occurrences of taxa in the wild.</rdfs:comment>

   </owl:Ontology>


   <!-- *************************************************
					O C C U R R E N C E   R E C O R D  
 		**************************************************** -->
   <!-- OccurrenceRecord -->
   <owl:Class rdf:ID="OccurrenceRecord">
      <rdfs:label>Occurrence Record</rdfs:label>
      <rdfs:comment>The record of the occurrence of a taxon in the wild. An OccurrenceRecord may be
         vouchered with one or more specimens.</rdfs:comment>
      <rdfs:subClassOf rdf:resource="http://rs.tdwg.org/ontology/Base#BaseThing"/>
      <rdfs:isDefinedBy rdf:resource="http://rs.tdwg.org/ontology/voc/OccurrenceRecord"/>
   </owl:Class>

   <!-- OccurrenceRecord::hasVoucher -->
   <owl:ObjectProperty rdf:ID="hasVoucher">
      <rdfs:label>Has Voucher</rdfs:label>
      <rdfs:comment>A voucher specimen for the occurrence record that may be used to confirm
         identity and other data about the record.</rdfs:comment>
      <rdfs:domain rdf:resource="#OccurrenceRecord"/>
      <rdfs:range rdf:resource="http://rs.tdwg.org/ontology/voc/Specimen#Specimen"/>
      <rdfs:isDefinedBy rdf:resource="http://rs.tdwg.org/ontology/voc/OccurrenceRecord"/>
      <dc:relation rdf:resource="http://rs.tdwg.org/ontology/voc/OccurrenceRecord#voucherString"/>
   </owl:ObjectProperty>

   <!-- OccurrenceRecord::voucherString -->
   <owl:DatatypeProperty rdf:ID="voucherString">
      <rdfs:label>Voucher String</rdfs:label>
      <rdfs:comment>A string representation of a voucher. May be used for a collector/observer
         number or other identifier in combination with or as a replacement for a link to voucher
         specimen by hasVoucher.</rdfs:comment>
      <rdfs:domain rdf:resource="#OccurrenceRecord"/>
      <rdfs:range rdf:resource="http://www.w3.org/2001/XMLSchema#string"/>
      <rdfs:isDefinedBy rdf:resource="http://rs.tdwg.org/ontology/voc/OccurrenceRecord"/>
      <tcom:darwinCoreEquivalence>Core:Collector</tcom:darwinCoreEquivalence>
      <dc:relation rdf:resource="http://rs.tdwg.org/ontology/voc/OccurrenceRecord#hasVoucher"/>
   </owl:DatatypeProperty>

   <!-- OccurrenceRecord::identifiedTo -->
   <owl:ObjectProperty rdf:ID="identifiedTo">
      <rdfs:label>Identified To</rdfs:label>
      <rdfs:comment>An identification for this occurrence record.</rdfs:comment>
      <rdfs:domain rdf:resource="#OccurrenceRecord"/>
      <rdfs:range rdf:resource="http://rs.tdwg.org/ontology/voc/OccurrenceRecord#Identification"/>
      <rdfs:isDefinedBy rdf:resource="http://rs.tdwg.org/ontology/voc/OccurrenceRecord"/>
      <dc:relation
         rdf:resource="http://rs.tdwg.org/ontology/voc/OccurrenceRecord#identifiedToString"/>
   </owl:ObjectProperty>

   <!-- OccurrenceRecord::identifiedToString -->
   <owl:DatatypeProperty rdf:ID="identifiedToString">
      <rdfs:label>Identified To String</rdfs:label>
      <rdfs:comment>An identification for this occurrence record as a string</rdfs:comment>
      <rdfs:domain rdf:resource="#OccurrenceRecord"/>
      <rdfs:range rdf:resource="http://www.w3.org/2001/XMLSchema#string"/>
      <rdfs:isDefinedBy rdf:resource="http://rs.tdwg.org/ontology/voc/OccurrenceRecord"/>
      <dc:relation rdf:resource="http://rs.tdwg.org/ontology/voc/OccurrenceRecord#identifiedTo"/>
   </owl:DatatypeProperty>

   <!-- OccurrenceRecord::derivedFrom -->
   <owl:ObjectProperty rdf:ID="derivedFrom">
      <rdfs:label>Derived From</rdfs:label>
      <rdfs:comment>This OccurrenceRecord has been derived from another occurrence record following
         some procedure that may be documented by the procedure property.</rdfs:comment>
      <rdfs:domain rdf:resource="#OccurrenceRecord"/>
      <rdfs:range rdf:resource="http://rs.tdwg.org/ontology/voc/OccurrenceRecord#OccurrenceRecord"/>
      <rdfs:isDefinedBy rdf:resource="http://rs.tdwg.org/ontology/voc/OccurrenceRecord"/>
   </owl:ObjectProperty>

   <!-- OccurrenceRecord::procedure -->
   <owl:ObjectProperty rdf:ID="procedure">
      <rdfs:label>Procedure</rdfs:label>
      <rdfs:comment>The procedure followed that generated this record perhaps by derivation from
         another record or from the voucher or other means.</rdfs:comment>
      <rdfs:domain rdf:resource="#OccurrenceRecord"/>
      <rdfs:range rdf:resource="http://rs.tdwg.org/ontology/voc/Procedure#Procedure"/>
      <rdfs:isDefinedBy rdf:resource="http://rs.tdwg.org/ontology/voc/OccurrenceRecord"/>
      <dc:relation
         rdf:resource="http://rs.tdwg.org/ontology/voc/OccurrenceRecord#procedureDescriptor"/>
   </owl:ObjectProperty>

   <!-- OccurrenceRecord::procedureDescriptor -->
   <owl:DatatypeProperty rdf:ID="procedureDescriptor">
      <rdfs:label>Procedure Descriptor</rdfs:label>
      <rdfs:comment>A string description of the procedure employed in generating this occurrence
         record. This may be interpreted in combination with and qualifying the procedure property.</rdfs:comment>
      <rdfs:domain rdf:resource="#OccurrenceRecord"/>
      <rdfs:range rdf:resource="http://www.w3.org/2001/XMLSchema#string"/>
      <rdfs:isDefinedBy rdf:resource="http://rs.tdwg.org/ontology/voc/OccurrenceRecord"/>
      <dc:relation rdf:resource="http://rs.tdwg.org/ontology/voc/OccurrenceRecord#procedure"/>
   </owl:DatatypeProperty>

   <!-- OccurrenceRecord::higherGeography -->
   <owl:DatatypeProperty rdf:ID="higherGeography">
      <rdfs:label>Higher Geography</rdfs:label>
      <rdfs:comment>The combination of all geographic elements less specific than locality. "Like"
         query operations on this element will search for a substring that might be in any of the
         higher geography elements.</rdfs:comment>
      <rdfs:domain rdf:resource="#OccurrenceRecord"/>
      <rdfs:range rdf:resource="http://www.w3.org/2001/XMLSchema#string"/>
      <rdfs:isDefinedBy rdf:resource="http://rs.tdwg.org/ontology/voc/OccurrenceRecord"/>
      <tcom:darwinCoreEquivalence>Core:HigherGeography</tcom:darwinCoreEquivalence>
   </owl:DatatypeProperty>

   <!-- OccurrenceRecord::continent -->
   <owl:DatatypeProperty rdf:ID="continent">
      <rdfs:label>Continent</rdfs:label>
      <rdfs:comment>The full, unabbreviated name of the continent on which the organism was
         collected or observed.</rdfs:comment>
      <rdfs:domain rdf:resource="#OccurrenceRecord"/>
      <rdfs:range rdf:resource="http://www.w3.org/2001/XMLSchema#string"/>
      <rdfs:isDefinedBy rdf:resource="http://rs.tdwg.org/ontology/voc/OccurrenceRecord"/>
      <tcom:darwinCoreEquivalence>Core:Continent</tcom:darwinCoreEquivalence>
   </owl:DatatypeProperty>


   <!-- OccurrenceRecord::waterBody -->
   <owl:DatatypeProperty rdf:ID="waterBody">
      <rdfs:label>Water Body</rdfs:label>
      <rdfs:comment>The full, unabbreviated name of the body of water in or over which the organism
         was collected or observed.</rdfs:comment>
      <rdfs:domain rdf:resource="#OccurrenceRecord"/>
      <rdfs:range rdf:resource="http://www.w3.org/2001/XMLSchema#string"/>
      <rdfs:isDefinedBy rdf:resource="http://rs.tdwg.org/ontology/voc/OccurrenceRecord"/>
      <tcom:darwinCoreEquivalence>Core:WaterBody</tcom:darwinCoreEquivalence>
   </owl:DatatypeProperty>


   <!-- OccurrenceRecord::islandGroup -->
   <owl:DatatypeProperty rdf:ID="islandGroup">
      <rdfs:label>Island Group</rdfs:label>
      <rdfs:comment>The full, unabbreviated name of the island group in which the organism was
         collected or observed.</rdfs:comment>
      <rdfs:domain rdf:resource="#OccurrenceRecord"/>
      <rdfs:range rdf:resource="http://www.w3.org/2001/XMLSchema#string"/>
      <rdfs:isDefinedBy rdf:resource="http://rs.tdwg.org/ontology/voc/OccurrenceRecord"/>
      <tcom:darwinCoreEquivalence>Core:IslandGroup</tcom:darwinCoreEquivalence>
   </owl:DatatypeProperty>

   <!-- OccurrenceRecord::island -->
   <owl:DatatypeProperty rdf:ID="island">
      <rdfs:label>Island</rdfs:label>
      <rdfs:comment>The full, unabbreviated name of the island on which the organism was collected
         or observed.</rdfs:comment>
      <rdfs:domain rdf:resource="#OccurrenceRecord"/>
      <rdfs:range rdf:resource="http://www.w3.org/2001/XMLSchema#string"/>
      <rdfs:isDefinedBy rdf:resource="http://rs.tdwg.org/ontology/voc/OccurrenceRecord"/>
      <tcom:darwinCoreEquivalence>Core:Island</tcom:darwinCoreEquivalence>
   </owl:DatatypeProperty>

   <!-- OccurrenceRecord::country -->
   <owl:DatatypeProperty rdf:ID="country">
      <rdfs:label>Country</rdfs:label>
      <rdfs:comment>The full, unabbreviated name of the country or major political unit in which the
         organism was collected or observed.</rdfs:comment>
      <rdfs:domain rdf:resource="#OccurrenceRecord"/>
      <rdfs:range rdf:resource="http://www.w3.org/2001/XMLSchema#string"/>
      <rdfs:isDefinedBy rdf:resource="http://rs.tdwg.org/ontology/voc/OccurrenceRecord"/>
      <tcom:darwinCoreEquivalence>Core:Country</tcom:darwinCoreEquivalence>
   </owl:DatatypeProperty>

   <!-- OccurrenceRecord::stateProvince -->
   <owl:DatatypeProperty rdf:ID="stateProvince">
      <rdfs:label>State Province</rdfs:label>
      <rdfs:comment>The full, unabbreviated name of the state, province, or region (i.e., the next
         smaller political region than Country) in which the organism was collected or observed. </rdfs:comment>
      <rdfs:domain rdf:resource="#OccurrenceRecord"/>
      <rdfs:range rdf:resource="http://www.w3.org/2001/XMLSchema#string"/>
      <rdfs:isDefinedBy rdf:resource="http://rs.tdwg.org/ontology/voc/OccurrenceRecord"/>
      <tcom:darwinCoreEquivalence>Core:StateProvince</tcom:darwinCoreEquivalence>
   </owl:DatatypeProperty>


   <!-- OccurrenceRecord::county -->
   <owl:DatatypeProperty rdf:ID="county">
      <rdfs:label>County</rdfs:label>
      <rdfs:comment>The full, unabbreviated name of the county, shire, or municipality (i.e., the
         next smaller political region than StateProvince) in which the organism was collected or
         observed.</rdfs:comment>
      <rdfs:domain rdf:resource="#OccurrenceRecord"/>
      <rdfs:range rdf:resource="http://www.w3.org/2001/XMLSchema#string"/>
      <rdfs:isDefinedBy rdf:resource="http://rs.tdwg.org/ontology/voc/OccurrenceRecord"/>
      <tcom:darwinCoreEquivalence>Core:County</tcom:darwinCoreEquivalence>
   </owl:DatatypeProperty>

   <!-- OccurrenceRecord::locality -->
   <owl:DatatypeProperty rdf:ID="locality">
      <rdfs:label>Locality</rdfs:label>
      <rdfs:comment>The full, unabbreviated name of the locality where the organism was collected or
         observed. This element need not contain geographic information provided in other geographic
         elements.</rdfs:comment>
      <rdfs:domain rdf:resource="#OccurrenceRecord"/>
      <rdfs:range rdf:resource="http://www.w3.org/2001/XMLSchema#string"/>
      <rdfs:isDefinedBy rdf:resource="http://rs.tdwg.org/ontology/voc/OccurrenceRecord"/>
      <tcom:darwinCoreEquivalence>Core:Locality</tcom:darwinCoreEquivalence>
   </owl:DatatypeProperty>


   <!-- OccurrenceRecord::minimumElevationInMeters -->
   <owl:DatatypeProperty rdf:ID="minimumElevationInMeters">
      <rdfs:label>Minimum Elevation In Meters</rdfs:label>
      <rdfs:comment>The minimum or actual elevation at which the collection or observation was made.
         Use negative values for locations below sea level. Examples: 75 (for an elevation of 100 +-
         25 meters). 100 (for an elevation between 100m and 200m).</rdfs:comment>
      <rdfs:domain rdf:resource="#OccurrenceRecord"/>
      <rdfs:range rdf:resource="http://www.w3.org/2001/XMLSchema#string"/>
      <rdfs:isDefinedBy rdf:resource="http://rs.tdwg.org/ontology/voc/OccurrenceRecord"/>
      <tcom:darwinCoreEquivalence>Core:MinimumElevationInMeters</tcom:darwinCoreEquivalence>
   </owl:DatatypeProperty>


   <!-- OccurrenceRecord::maximumElevationInMeters -->
   <owl:DatatypeProperty rdf:ID="maximumElevationInMeters">
      <rdfs:label>Maximum Elevation In Meters</rdfs:label>
      <rdfs:comment>The maximum or actual elevation at which the collection or observation was made.
         Use negative values for locations below sea level. Examples: Examples: 125 (for an
         elevation of 100 +- 25 meters). 200 (for an elevation between 100m and 200m).</rdfs:comment>
      <rdfs:domain rdf:resource="#OccurrenceRecord"/>
      <rdfs:range rdf:resource="http://www.w3.org/2001/XMLSchema#string"/>
      <rdfs:isDefinedBy rdf:resource="http://rs.tdwg.org/ontology/voc/OccurrenceRecord"/>
      <tcom:darwinCoreEquivalence>Core:MaximumElevationInMeters</tcom:darwinCoreEquivalence>
   </owl:DatatypeProperty>

   <!-- OccurrenceRecord::minimumDepthInMeters -->
   <owl:DatatypeProperty rdf:ID="minimumDepthInMeters">
      <rdfs:label>Minimum Depth In Meters</rdfs:label>
      <rdfs:comment>The minimum or actual depth at which the collection or observation was made. Use
         positive values for locations below the surface. Examples: 0 (for a depth of up to 10m). 50
         (for a depth between 50m and 100m).</rdfs:comment>
      <rdfs:domain rdf:resource="#OccurrenceRecord"/>
      <rdfs:range rdf:resource="http://www.w3.org/2001/XMLSchema#string"/>
      <rdfs:isDefinedBy rdf:resource="http://rs.tdwg.org/ontology/voc/OccurrenceRecord"/>
      <tcom:darwinCoreEquivalence>Core:MinimumDepthInMeters</tcom:darwinCoreEquivalence>
   </owl:DatatypeProperty>

   <!-- OccurrenceRecord::maximumDepthInMeters -->
   <owl:DatatypeProperty rdf:ID="maximumDepthInMeters">
      <rdfs:label>Maximum Depth In Meters</rdfs:label>
      <rdfs:comment>The maximum or actual depth at which the collection or observation was made. Use
         positive values for locations below the surface. Examples: 10 (for a depth of up to 10m).
         100 (for a depth between 50m and 100m).</rdfs:comment>
      <rdfs:domain rdf:resource="#OccurrenceRecord"/>
      <rdfs:range rdf:resource="http://www.w3.org/2001/XMLSchema#string"/>
      <rdfs:isDefinedBy rdf:resource="http://rs.tdwg.org/ontology/voc/OccurrenceRecord"/>
      <tcom:darwinCoreEquivalence>Core:MaximumDepthInMeters</tcom:darwinCoreEquivalence>
   </owl:DatatypeProperty>

   <!-- OccurrenceRecord::validDistributionFlag -->
   <owl:DatatypeProperty rdf:ID="validDistributionFlag">
      <rdfs:label>Valid Distribution Flag</rdfs:label>
      <rdfs:comment>A flag ("true" or "false") that indicates whether the locality information
         represents a valid distribution occurrence for a specimen. Specimens taken from captivity
         and showing the captive location should use the value "false".</rdfs:comment>
      <rdfs:domain rdf:resource="#OccurrenceRecord"/>
      <rdfs:range rdf:resource="http://www.w3.org/2001/XMLSchema#boolean"/>
      <rdfs:isDefinedBy rdf:resource="http://rs.tdwg.org/ontology/voc/OccurrenceRecord"/>
      <tcom:darwinCoreEquivalence>Core:ValidDistributionFlag</tcom:darwinCoreEquivalence>
   </owl:DatatypeProperty>

   <!-- OccurrenceRecord::earliestDateCollected -->
   <owl:DatatypeProperty rdf:ID="earliestDateCollected">
      <rdfs:label>Earliest Date Collected</rdfs:label>
      <rdfs:comment>The earliest date-time (Common Era calendar) in a date-time period during which
         an organism or group of organisms was collected or observed. If the event is recorded as
         occurring at a single date-time, populate both EarliestDateCollected and
         LatestDateCollected with the same value.</rdfs:comment>
      <rdfs:domain rdf:resource="#OccurrenceRecord"/>
      <rdfs:range rdf:resource="http://www.w3.org/2001/XMLSchema#dateTime"/>
      <rdfs:isDefinedBy rdf:resource="http://rs.tdwg.org/ontology/voc/OccurrenceRecord"/>
      <tcom:darwinCoreEquivalence>Core:EarliestDateCollected</tcom:darwinCoreEquivalence>
   </owl:DatatypeProperty>

   <!-- OccurrenceRecord::latestDateCollected -->
   <owl:DatatypeProperty rdf:ID="latestDateCollected">
      <rdfs:label>Latest Date Collected</rdfs:label>
      <rdfs:comment>The latest date-time (Common Era calendar) in a date-time period during which an
         organism or group of organisms was collected or observed. If the event is recorded as
         occurring at a single date-time, populate both EarliestDateCollected and
         LatestDateCollected with the same value.</rdfs:comment>
      <rdfs:domain rdf:resource="#OccurrenceRecord"/>
      <rdfs:range rdf:resource="http://www.w3.org/2001/XMLSchema#dateTime"/>
      <rdfs:isDefinedBy rdf:resource="http://rs.tdwg.org/ontology/voc/OccurrenceRecord"/>
      <tcom:darwinCoreEquivalence>Core:LatestDateCollected</tcom:darwinCoreEquivalence>
   </owl:DatatypeProperty>

   <!-- OccurrenceRecord::dayOfYear -->
   <owl:DatatypeProperty rdf:ID="dayOfYear">
      <rdfs:label>Day Of Year</rdfs:label>
      <rdfs:comment>The ordinal day of the year on which the object or observation was collected (1
         for January 1, 365 for December 31, except in a leap year, in which case it is 366). If the
         EarliestDateCollected and LatestDateCollected do not occur on the same day, do not populate
         DayOfYear.</rdfs:comment>
      <rdfs:domain rdf:resource="#OccurrenceRecord"/>
      <rdfs:range rdf:resource="http://www.w3.org/2001/XMLSchema#integer"/>
      <rdfs:isDefinedBy rdf:resource="http://rs.tdwg.org/ontology/voc/OccurrenceRecord"/>
      <tcom:darwinCoreEquivalence>Core:DayOfYear</tcom:darwinCoreEquivalence>
   </owl:DatatypeProperty>

   <!-- OccurrenceRecord::decimalLatitude -->
   <owl:DatatypeProperty rdf:ID="decimalLatitude">
      <rdfs:label>Decimal Latitude</rdfs:label>
      <rdfs:comment>The latitude of the location from which the organism or observation was
         collected, expressed in decimal degrees. Positive values are North of the Equator, negative
         values are South of the Equator.</rdfs:comment>
      <rdfs:domain rdf:resource="#OccurrenceRecord"/>
      <rdfs:range rdf:resource="http://www.w3.org/2001/XMLSchema#double"/>
      <rdfs:isDefinedBy rdf:resource="http://rs.tdwg.org/ontology/voc/OccurrenceRecord"/>
      <tcom:darwinCoreEquivalence>Geospatial:DecimalLatitude</tcom:darwinCoreEquivalence>
   </owl:DatatypeProperty>

   <!-- OccurrenceRecord::decimalLongitude -->
   <owl:DatatypeProperty rdf:ID="decimalLongitude">
      <rdfs:label>Decimal Longitude</rdfs:label>
      <rdfs:comment> The longitude of the location from which the organism or observation was
         collected, expressed in decimal degrees. Positive values are East of the Greenwich
         Meridian, negative values are West of the Greenwich Meridian.</rdfs:comment>
      <rdfs:domain rdf:resource="#OccurrenceRecord"/>
      <rdfs:range rdf:resource="http://www.w3.org/2001/XMLSchema#double"/>
      <rdfs:isDefinedBy rdf:resource="http://rs.tdwg.org/ontology/voc/OccurrenceRecord"/>
      <tcom:darwinCoreEquivalence>Geospatial:DecimalLongitude</tcom:darwinCoreEquivalence>
   </owl:DatatypeProperty>

   <!-- OccurrenceRecord::geodeticDatum -->
   <owl:DatatypeProperty rdf:ID="geodeticDatum">
      <rdfs:label>Geodetic Datum</rdfs:label>
      <rdfs:comment>The geodetic datum to which the latitude and longitude refer. If not known, use
         "not recorded". This concept should be vocabulary-controlled.</rdfs:comment>
      <rdfs:domain rdf:resource="#OccurrenceRecord"/>
      <rdfs:range rdf:resource="http://www.w3.org/2001/XMLSchema#string"/>
      <rdfs:isDefinedBy rdf:resource="http://rs.tdwg.org/ontology/voc/OccurrenceRecord"/>
      <tcom:darwinCoreEquivalence>Geospatial:GeodeticDatum</tcom:darwinCoreEquivalence>
   </owl:DatatypeProperty>


   <!-- OccurrenceRecord::coordinateUncertaintyInMeters -->
   <owl:DatatypeProperty rdf:ID="coordinateUncertaintyInMeters">
      <rdfs:label>Coordinate Uncertainty In Meters</rdfs:label>
      <rdfs:comment>The upper limit of the distance (in meters) from the given latitude and
         longitude describing a circle within which the whole of the described locality lies. Leave
         the value empty if the uncertainty is unknown, cannot be estimated, or is not applicable
         (because there are no coordinates). The value should be greater than zero. </rdfs:comment>
      <rdfs:domain rdf:resource="#OccurrenceRecord"/>
      <rdfs:range rdf:resource="http://www.w3.org/2001/XMLSchema#double"/>
      <rdfs:isDefinedBy rdf:resource="http://rs.tdwg.org/ontology/voc/OccurrenceRecord"/>
      <tcom:darwinCoreEquivalence>Geospatial:CoordinateUncertaintyInMeters</tcom:darwinCoreEquivalence>
   </owl:DatatypeProperty>

   <!-- OccurrenceRecord::pointRadiusSpatialFit -->
   <owl:DatatypeProperty rdf:ID="pointRadiusSpatialFit">
      <rdfs:label>Point Radius Spatial Fit</rdfs:label>
      <rdfs:comment>A measure of how well the circle defined by the coordinates and uncertainty
         match the original spatial representation, as a ratio of the area of the circle to the area
         of the original spatial representation. Legal values are 0, greater than or equal to 1. A
         value of 1 is an exact match or 100% overlap. A value of 0 should be used if the given
         georeference does not completely contain the original representation. The
         PointRadiusSpatialFit is undefined if the original representation is a point without
         uncertainty and the given georeference is not that same point (without uncertainty). If
         both the original and the given georeference are the same point, the PointRadiusSpatialFit
         is 1. Detailed explanations with graphical examples can be found in the Guide to Best
         Practices for Georeferencing (Chapman and Wieczorek, eds. 2006)
         http://www.gbif.org/prog/digit/Georeferencing.</rdfs:comment>
      <rdfs:domain rdf:resource="#OccurrenceRecord"/>
      <rdfs:range rdf:resource="http://www.w3.org/2001/XMLSchema#double"/>
      <rdfs:isDefinedBy rdf:resource="http://rs.tdwg.org/ontology/voc/OccurrenceRecord"/>
      <tcom:darwinCoreEquivalence>Geospatial:pointRadiusSpatialFit</tcom:darwinCoreEquivalence>
   </owl:DatatypeProperty>

   <!-- OccurrenceRecord::georeferenceProtocol -->
   <owl:DatatypeProperty rdf:ID="georeferenceProtocol">
      <rdfs:label>Georeference Protocol</rdfs:label>
      <rdfs:comment>A reference to the methods used for determining the coordinates and
         uncertainties. Example: "http://manisnet.org/GeorefGuide.html".</rdfs:comment>
      <rdfs:domain rdf:resource="#OccurrenceRecord"/>
      <rdfs:range rdf:resource="http://www.w3.org/2001/XMLSchema#string"/>
      <rdfs:isDefinedBy rdf:resource="http://rs.tdwg.org/ontology/voc/OccurrenceRecord"/>
      <tcom:darwinCoreEquivalence>Geospatial:GeoreferenceProtocol</tcom:darwinCoreEquivalence>
   </owl:DatatypeProperty>


   <!-- OccurrenceRecord::georeferenceSources -->
   <owl:DatatypeProperty rdf:ID="georeferenceSources">
      <rdfs:label>Georeference Sources</rdfs:label>
      <rdfs:comment>A list of maps, gazetteers or other resources used to georeference the locality.
         The content of this concept is meant to be specific enough to allow anyone in the future to
         use the same resource to georeference the same locality. Example: "USGS 1:24000 Florence
         Montana Quad".</rdfs:comment>
      <rdfs:domain rdf:resource="#OccurrenceRecord"/>
      <rdfs:range rdf:resource="http://www.w3.org/2001/XMLSchema#string"/>
      <rdfs:isDefinedBy rdf:resource="http://rs.tdwg.org/ontology/voc/OccurrenceRecord"/>
      <tcom:darwinCoreEquivalence>Geospatial:GeoreferenceSources</tcom:darwinCoreEquivalence>
   </owl:DatatypeProperty>


   <!-- OccurrenceRecord::georeferenceVerificationStatus -->
   <owl:DatatypeProperty rdf:ID="georeferenceVerificationStatus">
      <rdfs:label>Georeference Sources</rdfs:label>
      <rdfs:comment>A categorical description of the extent to which the georeference has been
         verified to represent the location where the specimen or observation was collected. This
         element should be vocabulary-controlled. Examples: "requires verification", "verified by
         collector", "verified by curator".</rdfs:comment>
      <rdfs:domain rdf:resource="#OccurrenceRecord"/>
      <rdfs:range rdf:resource="http://www.w3.org/2001/XMLSchema#string"/>
      <rdfs:isDefinedBy rdf:resource="http://rs.tdwg.org/ontology/voc/OccurrenceRecord"/>
      <tcom:darwinCoreEquivalence>Geospatial:GeoreferenceVerificationStatus</tcom:darwinCoreEquivalence>
   </owl:DatatypeProperty>

   <!-- OccurrenceRecord::georeferenceRemarks -->
   <owl:DatatypeProperty rdf:ID="georeferenceRemarks">
      <rdfs:label>Georeference Remarks</rdfs:label>
      <rdfs:comment>Comments about the spatial description determination, explaining assumptions
         made in addition or opposition to the those formalized in the method referred to in
         GeoreferenceProtocol.</rdfs:comment>
      <rdfs:domain rdf:resource="#OccurrenceRecord"/>
      <rdfs:range rdf:resource="http://www.w3.org/2001/XMLSchema#string"/>
      <rdfs:isDefinedBy rdf:resource="http://rs.tdwg.org/ontology/voc/OccurrenceRecord"/>
      <tcom:darwinCoreEquivalence>Geospatial:GeoreferenceRemarks</tcom:darwinCoreEquivalence>
   </owl:DatatypeProperty>

   <!-- OccurrenceRecord::wktFootprint -->
   <owl:DatatypeProperty rdf:ID="wktFootprint">
      <rdfs:label>Well-Known Text Footprint</rdfs:label>
      <rdfs:comment>A Well-Known Text (WKT; see http://en.wikipedia.org/wiki/Well-known_text)
         representation of the the shape (footprint) that defines the location of the occurrence.
         Example: the one-degree boundin box with opposite corners at (longitude=10, latitude=20)
         and (longitude=11, latitude=21) would be expressed in well-known text as POLYGON ((10 20,
         11 20, 11 21, 10 21, 10 20))</rdfs:comment>
      <rdfs:domain rdf:resource="#OccurrenceRecord"/>
      <rdfs:range rdf:resource="http://www.w3.org/2001/XMLSchema#string"/>
      <rdfs:isDefinedBy rdf:resource="http://rs.tdwg.org/ontology/voc/OccurrenceRecord"/>
      <tcom:darwinCoreEquivalence>Geospatial:WKTFootprint</tcom:darwinCoreEquivalence>
   </owl:DatatypeProperty>

   <!-- OccurrenceRecord::footprintSpatialFit -->
   <owl:DatatypeProperty rdf:ID="footprintSpatialFit">
      <rdfs:label>Footprint Spatial Fit</rdfs:label>
      <rdfs:comment>A measure of how well the geometry expressed in the footprint match the original
         spatial representation, as a ratio of the area of the footprint given to the area of the
         original spatial representation. Legal values are 0, greater than or equal to 1. A value of
         1 is an exact match or 100% overlap. A value of 0 should be used if the given georeference
         does not completely contain the original representation. The FootprintSpatialFit is
         undefined if the original representation is a point without uncertainty and the given
         georeference is not that same point (without uncertainty). If both the original and the
         given georeference are the same point, the FootprintSpatialFit is 1. Detailed explanations
         with graphical examples can be found in the Guide to Best Practices for Georeferencing
         (Chapman and Wieczorek, eds. 2006). http://www.gbif.org/prog/digit/Georeferencing</rdfs:comment>
      <rdfs:domain rdf:resource="#OccurrenceRecord"/>
      <rdfs:range rdf:resource="http://www.w3.org/2001/XMLSchema#double"/>
      <rdfs:isDefinedBy rdf:resource="http://rs.tdwg.org/ontology/voc/OccurrenceRecord"/>
      <tcom:darwinCoreEquivalence>Geospatial:FootprintSpatialFit</tcom:darwinCoreEquivalence>
   </owl:DatatypeProperty>

   <!-- OccurrenceRecord::value -->
   <owl:DatatypeProperty rdf:ID="value">
      <rdfs:label>Value</rdfs:label>
      <rdfs:comment>An OccurrenceRecord may represent more that just the presence of an instance of
         a taxon in the wild. If the occurrence is the result of a survey there may well be a
         quantitative measure associated with the record such as a count or frequency. In the most
         simple case this property may contain the integer 0 indicating a lack of occurrence. If
         this property is present then its meaning (including units) should be interpreted in terms
         of the value of the procedure property. The associated valueConfidence property is provided
         to hold indication of error or deviation - again dependent on the procedure followed.</rdfs:comment>
      <rdfs:domain rdf:resource="#OccurrenceRecord"/>
      <rdfs:range rdf:resource="http://www.w3.org/2001/XMLSchema#double"/>
      <rdfs:isDefinedBy rdf:resource="http://rs.tdwg.org/ontology/voc/OccurrenceRecord"/>
      <tcom:darwinCoreEquivalence>FIXME </tcom:darwinCoreEquivalence>
      <dc:relation rdf:resource="http://rs.tdwg.org/ontology/voc/OccurrenceRecord#valueConfidence"/>
   </owl:DatatypeProperty>

   <!-- OccurrenceRecord::valueConfidence -->
   <owl:DatatypeProperty rdf:ID="valueConfidence">
      <rdfs:label>Value Confidence</rdfs:label>
      <rdfs:comment>This property should be interpreted in association with the value property. It
         provides a measure of error associated with that measurement in the context of the
         procedure followed in the procedure property.</rdfs:comment>
      <rdfs:domain rdf:resource="#OccurrenceRecord"/>
      <rdfs:range rdf:resource="http://www.w3.org/2001/XMLSchema#double"/>
      <rdfs:isDefinedBy rdf:resource="http://rs.tdwg.org/ontology/voc/OccurrenceRecord"/>
      <tcom:darwinCoreEquivalence>No equivalent</tcom:darwinCoreEquivalence>
      <dc:relation rdf:resource="http://rs.tdwg.org/ontology/voc/OccurrenceRecord#value"/>
   </owl:DatatypeProperty>


   <!-- *************************************************
            I D E N T I F I C A T I O N  
            **************************************************** -->

   <!-- Identification -->
   <owl:Class rdf:ID="Identification">
      <rdfs:label>Identification</rdfs:label>
      <rdfs:comment> The identification or determination of the occurrence of a taxon to a specific
         taxon.</rdfs:comment>
      <rdfs:subClassOf rdf:resource="http://rs.tdwg.org/ontology/Base#BaseThing"/>
      <rdfs:isDefinedBy rdf:resource="http://rs.tdwg.org/ontology/voc/OccurrenceRecord"/>
   </owl:Class>

   <!-- Identification::expert -->
   <owl:ObjectProperty rdf:ID="expert">
      <rdfs:label>Expert</rdfs:label>
      <rdfs:comment>The person who made this identification. May also be represented by
         expertString. The 'Who' of and identification.</rdfs:comment>
      <rdfs:domain rdf:resource="#Identification"/>
      <rdfs:range rdf:resource="http://rs.tdwg.org/ontology/voc/Person#Person"/>
      <rdfs:isDefinedBy rdf:resource="http://rs.tdwg.org/ontology/voc/OccurrenceRecord"/>
      <dc:relation rdf:resource="http://rs.tdwg.org/ontology/voc/OccurrenceRecord#expertName"/>
   </owl:ObjectProperty>

   <!-- Identification::expertName -->
   <owl:DatatypeProperty rdf:ID="expertName">
      <rdfs:label>Expert Name</rdfs:label>
      <rdfs:comment>A string representation of the person or agent that identified this occurrence
         record. This may be interpreted in combination with method property - particularly if the
         method is automated and no human was present.</rdfs:comment>
      <rdfs:domain rdf:resource="#Identification"/>
      <rdfs:range rdf:resource="http://www.w3.org/2001/XMLSchema#string"/>
      <rdfs:isDefinedBy rdf:resource="http://rs.tdwg.org/ontology/voc/OccurrenceRecord"/>
      <dc:relation rdf:resource="http://rs.tdwg.org/ontology/voc/OccurrenceRecord#expert"/>
   </owl:DatatypeProperty>


   <!-- Identification::occurrence -->
   <owl:ObjectProperty rdf:ID="occurrence">
      <rdfs:label>occurrence</rdfs:label>
      <rdfs:comment> The OccurrenceRecord that is identified by this identification. The 'What' of
         an identification. This property is usually omitted when and identification object is
         embedded within an OccurrenceRecord when the subject of the identification is implied. </rdfs:comment>
      <rdfs:domain rdf:resource="#Identification"/>
      <rdfs:range rdf:resource="http://rs.tdwg.org/ontology/voc/OccurrenceRecord#OccurrenceRecord"/>
      <rdfs:isDefinedBy rdf:resource="http://rs.tdwg.org/ontology/voc/OccurrenceRecord"/>
   </owl:ObjectProperty>


   <!-- Identification::date -->
   <owl:DatatypeProperty rdf:ID="date">
      <rdfs:label>date</rdfs:label>
      <rdfs:comment> The date and time the identification occurred. The 'When' of an identification.</rdfs:comment>
      <rdfs:domain rdf:resource="#Identification"/>
      <rdfs:range rdf:resource="http://www.w3.org/2001/XMLSchema#dateTime"/>
      <rdfs:isDefinedBy rdf:resource="http://rs.tdwg.org/ontology/voc/OccurrenceRecord"/>
   </owl:DatatypeProperty>

   <!-- Identification::location -->
   <owl:DatatypeProperty rdf:ID="location">
      <rdfs:label>location</rdfs:label>
      <rdfs:comment> The location the identification took place. The 'Where' of an identification.</rdfs:comment>
      <rdfs:domain rdf:resource="#Identification"/>
      <rdfs:range rdf:resource="http://www.w3.org/2001/XMLSchema#string"/>
      <rdfs:isDefinedBy rdf:resource="http://rs.tdwg.org/ontology/voc/OccurrenceRecord"/>
   </owl:DatatypeProperty>

   <!-- Identification::method -->
   <owl:ObjectProperty rdf:ID="method">
      <rdfs:label>Method</rdfs:label>
      <rdfs:comment> The procedure used to identify the occurrence. The 'How' of an identification.</rdfs:comment>
      <rdfs:domain rdf:resource="#Identification"/>
      <rdfs:range rdf:resource="http://rs.tdwg.org/ontology/voc/Procedure#Procedure"/>
      <rdfs:isDefinedBy rdf:resource="http://rs.tdwg.org/ontology/voc/OccurrenceRecord"/>
      <dc:relation rdf:resource="http://rs.tdwg.org/ontology/voc/OccurrenceRecord#methodDescriptor"
      />
   </owl:ObjectProperty>

   <!-- Identification::methodDescriptor -->
   <owl:DatatypeProperty rdf:ID="methodDescriptor">
      <rdfs:label>Method Descriptor</rdfs:label>
      <rdfs:comment>A string description of the method employed in the identification. This may be
         interpreted in combination with and qualifying the method property.</rdfs:comment>
      <rdfs:domain rdf:resource="#Identification"/>
      <rdfs:range rdf:resource="http://www.w3.org/2001/XMLSchema#string"/>
      <rdfs:isDefinedBy rdf:resource="http://rs.tdwg.org/ontology/voc/OccurrenceRecord"/>
      <dc:relation rdf:resource="http://rs.tdwg.org/ontology/voc/OccurrenceRecord#method"/>
   </owl:DatatypeProperty>


   <!-- Identification::confidence -->
   <owl:DatatypeProperty rdf:ID="confidence">
      <rdfs:label>Confidence</rdfs:label>
      <rdfs:comment>A measure of the confidence that the identification is correct. By default (in
         the absence of a method field) this should be interpreted as 0 = no confidence and 1 =
         total confidence but other interpretations may be appropriate depending on the value of the
         method field.</rdfs:comment>
      <rdfs:domain rdf:resource="#Identification"/>
      <rdfs:range rdf:resource="http://www.w3.org/2001/XMLSchema#double"/>
      <rdfs:isDefinedBy rdf:resource="http://rs.tdwg.org/ontology/voc/OccurrenceRecord"/>
      <tcom:darwinCoreEquivalence>No equivalent</tcom:darwinCoreEquivalence>
      <dc:relation rdf:resource="http://rs.tdwg.org/ontology/voc/OccurrenceRecord#value"/>
   </owl:DatatypeProperty>

   <!-- Identification::taxon -->
   <owl:ObjectProperty rdf:ID="taxon">
      <rdfs:label>Taxon</rdfs:label>
      <rdfs:comment>The TaxonConcept this occurrence is identified to.</rdfs:comment>
      <rdfs:domain rdf:resource="#Identification"/>
      <rdfs:range rdf:resource="http://rs.tdwg.org/ontology/voc/TaxonConcept#TaxonConcept"/>
      <rdfs:isDefinedBy rdf:resource="http://rs.tdwg.org/ontology/voc/OccurrenceRecord"/>
      <tcom:darwinCoreEquivalence>No equivalent</tcom:darwinCoreEquivalence>
      <dc:relation rdf:resource="http://rs.tdwg.org/ontology/voc/OccurrenceRecord#taxonName"/>
   </owl:ObjectProperty>

   <!-- Identification::taxonName -->
   <owl:DatatypeProperty rdf:ID="taxonName">
      <rdfs:label>Taxon Name</rdfs:label>
      <rdfs:comment>A string representation of the TaxonConcept this occurrence is identified to. Be
         aware that using a Taxon Name in here without qualifying in what sense it is used is
         imprecise. Some indication of the taxonomic monograph or treatment followed is important
         when available. Populate the taxon property whenever possible.</rdfs:comment>
      <rdfs:domain rdf:resource="#Identification"/>
      <rdfs:range rdf:resource="http://www.w3.org/2001/XMLSchema#string"/>
      <rdfs:isDefinedBy rdf:resource="http://rs.tdwg.org/ontology/voc/OccurrenceRecord"/>
      <dc:relation rdf:resource="http://rs.tdwg.org/ontology/voc/OccurrenceRecord#taxon"/>
   </owl:DatatypeProperty>

   <!-- Identification::ofOccurrenceRecord -->
   <owl:ObjectProperty rdf:ID="ofOccurrenceRecord">
      <rdfs:label>ofOccurrenceRecord</rdfs:label>
      <rdfs:comment>The OccurrenceRecord that this Identification is of. This property is used when
         the Indentification is 'free standing' and not the target of a
         OccurrenceRecord::identifiedTo property.</rdfs:comment>
      <rdfs:domain rdf:resource="#Identification"/>
      <rdfs:range rdf:resource="http://rs.tdwg.org/ontology/voc/OccurrenceRecord#OccurrenceRecord"/>
      <rdfs:isDefinedBy rdf:resource="http://rs.tdwg.org/ontology/voc/OccurrenceRecord"/>
   </owl:ObjectProperty>

   <!-- Identification::verbatimDet -->
   <owl:DatatypeProperty rdf:ID="verbatimDet">
      <rdfs:label>Verbatim Det</rdfs:label>
      <rdfs:comment>The verbatim text of an identification. For example the text of a determination
         slip attached to a herbarium specimen.</rdfs:comment>
      <rdfs:domain rdf:resource="#Identification"/>
      <rdfs:range rdf:resource="http://www.w3.org/2001/XMLSchema#string"/>
      <rdfs:isDefinedBy rdf:resource="http://rs.tdwg.org/ontology/voc/OccurrenceRecord"/>
   </owl:DatatypeProperty>

</rdf:RDF>
