<?xml version="1.0" encoding="UTF-8"?>
<!-- $Author: MarkusDoering $ -->

<rdf:RDF xmlns:rdf="http://www.w3.org/1999/02/22-rdf-syntax-ns#"
   xmlns:rdfs="http://www.w3.org/2000/01/rdf-schema#"
   xmlns:owl="http://www.w3.org/2002/07/owl#"
   xmlns:dc="http://purl.org/dc/elements/1.1/"
   xmlns:dcterms="http://purl.org/dc/terms/"
   xmlns:tbase="http://rs.tdwg.org/ontology/Base#"
   xmlns:tcore="http://rs.tdwg.org/ontology/Core#"
   xmlns:tcom="http://rs.tdwg.org/ontology/voc/Common#"
   xmlns:spm="http://rs.tdwg.org/ontology/voc/SpeciesProfileModel#"
   xmlns="http://rs.tdwg.org/ontology/voc/SpeciesProfileModel#"
   xml:base="http://rs.tdwg.org/ontology/voc/SpeciesProfileModel">

   <owl:Ontology rdf:about="http://rs.tdwg.org/ontology/voc/SpeciesProfileModel">
      <dc:title>TDWG SpeciesProfileModel LSID Ontology</dc:title>
      <dc:creator>Roger Hyam</dc:creator>
      <dc:publisher>TDWG Biodiversity Information Standards</dc:publisher>
      <dcterms:issued>2007-04-17</dcterms:issued>
      <dcterms:modified>2015-07-01</dcterms:modified>
      <dc:description>Vocabulary for exchanging data about taxa.</dc:description>

      <owl:versionInfo>0.4</owl:versionInfo>
      <owl:deprecated rdf:datatype="http://www.w3.org/2001/XMLSchema#boolean">true</owl:deprecated>
      <rdfs:comment>This ontology is no longer under development and is no longer recommended for use.  See https://github.com/tdwg/ontology for information about recommended replacements.</rdfs:comment>
      <rdfs:seeAlso rdf:resource="https://raw.githubusercontent.com/tdwg/ontology/master/replacements.rdf"/>

   </owl:Ontology>


   <!-- *************************************************
					T A X O N    D A T A    M O D E L
 	**************************************************** -->
   <!-- SpeciesProfileModel -->
   <owl:Class rdf:ID="SpeciesProfileModel">
      <rdfs:label>Species Profile Model</rdfs:label>
      <rdfs:comment>A set of information about a taxon.</rdfs:comment>
      <rdfs:isDefinedBy rdf:resource="http://rs.tdwg.org/ontology/voc/SpeciesProfileModel"/>
      <rdfs:subClassOf rdf:resource="http://rs.tdwg.org/ontology/Core#Description"/>
   </owl:Class>

   <!-- SpeciesProfileModel::aboutTaxon -->
   <owl:ObjectProperty rdf:ID="aboutTaxon">
      <rdfs:label>About Taxon</rdfs:label>
      <rdfs:comment>The taxon this information is about.</rdfs:comment>
      <rdfs:domain rdf:resource="#SpeciesProfileModel"/>
      <rdfs:range rdf:resource="http://rs.tdwg.org/ontology/voc/TaxonConcept#TaxonConcept"/>
      <rdfs:isDefinedBy rdf:resource="http://rs.tdwg.org/ontology/voc/SpeciesProfileModel"/>
   </owl:ObjectProperty>


   <!-- SpeciesProfileModel::hasInformation -->
   <owl:ObjectProperty rdf:ID="hasInformation">
      <rdfs:label>Has Information</rdfs:label>
      <rdfs:comment>A piece of information about this taxon.</rdfs:comment>
      <rdfs:domain rdf:resource="#SpeciesProfileModel"/>
      <rdfs:range rdf:resource="http://rs.tdwg.org/ontology/voc/SpeciesProfileModel#InfoItem"/>
      <rdfs:isDefinedBy rdf:resource="http://rs.tdwg.org/ontology/voc/SpeciesProfileModel"/>
   </owl:ObjectProperty>

   <!-- *************************************************
          I N F O   I T E M
      **************************************************** -->
   <!-- InfoItem -->
   <owl:Class rdf:ID="InfoItem">
      <rdfs:label>Information Item</rdfs:label>
      <rdfs:comment>A piece of information</rdfs:comment>
      <rdfs:subClassOf rdf:resource="http://rs.tdwg.org/ontology/Core#Description"/>
      <rdfs:isDefinedBy rdf:resource="http://rs.tdwg.org/ontology/voc/SpeciesProfileModel"/>
   </owl:Class>

   <!-- InfoItem::hasContent -->
   <owl:DatatypeProperty rdf:ID="hasContent">
      <rdfs:label>Has Content</rdfs:label>
      <rdfs:comment>A information about a taxon in the form of a string. Should be interpreted in combination with the type of the InfoItem</rdfs:comment>
      <rdfs:domain rdf:resource="#InfoItem"/>
      <rdfs:range rdf:resource="http://www.w3.org/2001/XMLSchema#string"/>
      <rdfs:isDefinedBy rdf:resource="http://rs.tdwg.org/ontology/voc/SpeciesProfileModel"/>
   </owl:DatatypeProperty>

   <!-- InfoItem::hasValue -->
   <owl:ObjectProperty rdf:ID="hasValue">
      <rdfs:label>Has Content</rdfs:label>
      <rdfs:comment>A information about a taxon in the form of a controlled vocabulary term.</rdfs:comment>
      <rdfs:domain rdf:resource="#InfoItem"/>
      <rdfs:range rdf:resource="http://rs.tdwg.org/ontology/Base#DefinedTerm"/>
      <rdfs:isDefinedBy rdf:resource="http://rs.tdwg.org/ontology/voc/SpeciesProfileModel"/>
   </owl:ObjectProperty>
   
   <!-- InfoItem::context -->
   <owl:DatatypeProperty rdf:ID="context">
      <rdfs:label>context</rdfs:label>
      <rdfs:comment>A string representation of when this information is valid.</rdfs:comment>
      <rdfs:domain rdf:resource="#InfoItem"/>
      <rdfs:range rdf:resource="http://www.w3.org/2001/XMLSchema#string"/>
      <rdfs:isDefinedBy rdf:resource="http://rs.tdwg.org/ontology/voc/SpeciesProfileModel"/>
   </owl:DatatypeProperty>

   <!-- InfoItem::category -->
   <owl:DatatypeProperty rdf:ID="category">
      <rdfs:label>category</rdfs:label>
      <rdfs:comment>A mechanism for indicating the category of information this info item is about. [There is currently a debate about whether this is better done by subclassing the InfoItem or by 'tagging' it with a type or category or both.]</rdfs:comment>
      <rdfs:domain rdf:resource="#InfoItem"/>
      <rdfs:range rdf:resource="http://www.w3.org/2001/XMLSchema#string"/>
      <rdfs:isDefinedBy rdf:resource="http://rs.tdwg.org/ontology/voc/SpeciesProfileModel"/>
   </owl:DatatypeProperty>

   <!-- InfoItem::contextValue -->
   <owl:ObjectProperty rdf:ID="contextValue">
      <rdfs:label>Context Value</rdfs:label>
      <rdfs:comment>An indication of when this information is valid according to a controlled vocabulary.</rdfs:comment>
      <rdfs:domain rdf:resource="#InfoItem"/>
      <rdfs:range rdf:resource="http://rs.tdwg.org/ontology/Base#DefinedTerm"/>
      <rdfs:isDefinedBy rdf:resource="http://rs.tdwg.org/ontology/voc/SpeciesProfileModel"/>
   </owl:ObjectProperty>


   <!-- InfoItem::contextOccurrence -->
   <owl:ObjectProperty rdf:ID="contextOccurrence">
      <rdfs:label>Context Occurrence</rdfs:label>
      <rdfs:comment>An indication of when this information is valid according to a geospatial data.</rdfs:comment>
      <rdfs:domain rdf:resource="#InfoItem"/>
      <rdfs:range rdf:resource="http://rs.tdwg.org/ontology/voc/OccurrenceRecord#OccurrenceRecord"/>
      <rdfs:isDefinedBy rdf:resource="http://rs.tdwg.org/ontology/voc/SpeciesProfileModel"/>
   </owl:ObjectProperty>


   <!-- InfoItem::associatedTaxon -->
   <owl:ObjectProperty rdf:ID="associatedTaxon">
      <rdfs:label>Associated Taxon</rdfs:label>
      <rdfs:comment>Another taxon associated with this taxon and this piece of information e.g. a parasite or prey</rdfs:comment>
      <rdfs:domain rdf:resource="#InfoItem"/>
      <rdfs:range rdf:resource="http://rs.tdwg.org/ontology/voc/TaxonConcept#TaxonConcept"/>
      <rdfs:isDefinedBy rdf:resource="http://rs.tdwg.org/ontology/voc/SpeciesProfileModel"/>
   </owl:ObjectProperty>

</rdf:RDF>
