<?xml version="1.0" encoding="UTF-8"?>
<!-- $Author: MarkusDoering $ -->

<rdf:RDF xmlns:rdf="http://www.w3.org/1999/02/22-rdf-syntax-ns#"
   xmlns:rdfs="http://www.w3.org/2000/01/rdf-schema#" xmlns:owl="http://www.w3.org/2002/07/owl#"
   xmlns:dc="http://purl.org/dc/elements/1.1/" xmlns:dcterms="http://purl.org/dc/terms/"
   xmlns:tbase="http://rs.tdwg.org/ontology/Base#" xmlns:tp="http://rs.tdwg.org/ontology/Person#"
   xml:base="http://rs.tdwg.org/ontology/voc/Team"
   xmlns:tt="http://rs.tdwg.org/ontology/voc/Team#"
   xmlns="http://rs.tdwg.org/ontology/voc/Team#">

   <owl:Ontology rdf:about="http://rs.tdwg.org/ontology/voc/Team">
      <dc:title>TDWG Team LSID Ontology</dc:title>
      <dc:creator>Roger Hyam</dc:creator>
      <dc:publisher>TDWG Biodiversity Information Standards</dc:publisher>
      <dcterms:issued>2006-11-27</dcterms:issued>
      <dcterms:modified>$Date: 2007-08-15 14:05:50 +0100 (Wed, 15 Aug 2007) $</dcterms:modified>
      <dc:description>Ontology describing the metadata returned for LSIDs that are used for Teams -
         collections of actors. </dc:description>

      <owl:versionInfo>0.2 - [SVN $Rev: 1294 $]</owl:versionInfo>

      <rdfs:comment rdf:parseType="Literal">A team is a collection of Actors (TeamMemebers) who may
         have roles and positions.</rdfs:comment>

   </owl:Ontology>


   <!-- *****************************************
					T E A M 
 		******************************************* -->
   <!-- Team -->
   <owl:Class rdf:ID="Team">
      <rdfs:label>Team</rdfs:label>
      <rdfs:comment>A team is a collection of Actors (TeamMembers) who may have roles and positions.</rdfs:comment>
      <rdfs:subClassOf rdf:resource="http://rs.tdwg.org/ontology/Core#Team"/>
      <rdfs:isDefinedBy rdf:resource="http://rs.tdwg.org/ontology/voc/Team"/>
   </owl:Class>
   
   <!-- Team::name -->
   <owl:DatatypeProperty rdf:ID="name">
      <rdfs:label>Name</rdfs:label>
      <rdfs:comment>A name for the team.</rdfs:comment>
      <rdfs:domain rdf:resource="#Team"/>
      <rdfs:range rdf:resource="http://www.w3.org/2001/XMLSchema#string"/>
      <rdfs:isDefinedBy rdf:resource="http://rs.tdwg.org/ontology/voc/Team"/>
   </owl:DatatypeProperty>

   <!-- Team::hasMember -->
   <owl:ObjectProperty rdf:ID="hasMember">
      <rdfs:label>Has Member</rdfs:label>
      <rdfs:comment>A member of this team. This property repeats to hold each member.</rdfs:comment>
      <rdfs:domain rdf:resource="#Team"/>
      <rdfs:range rdf:resource="http://rs.tdwg.org/ontology/voc/Team#TeamMember"/>
      <rdfs:isDefinedBy rdf:resource="http://rs.tdwg.org/ontology/voc/Team"/>
   </owl:ObjectProperty>

   <!-- Team::contactDetails -->
   <owl:ObjectProperty rdf:ID="contactDetails">
      <rdfs:label>contactDetails</rdfs:label>
      <rdfs:comment>A link to an object that contains contact information,
         (such as postal address, email address and phone number) for this team. </rdfs:comment>
      <rdfs:domain rdf:resource="#Team"/>
      <rdfs:range rdf:resource="http://rs.tdwg.org/ontology/voc/ContactDetails#ContactDetails"/>
      <rdfs:isDefinedBy rdf:resource="http://rs.tdwg.org/ontology/voc/Team"/>
   </owl:ObjectProperty>
   
   <!-- *****************************************
      T E A M   M E M B E R 
      ******************************************* -->
   <!-- TeamMember -->
   <owl:Class rdf:ID="TeamMember">
      <rdfs:label>Team Member</rdfs:label>
      <rdfs:comment>A representation of the role and position of an actor (Person etc) within a
         team.</rdfs:comment>
      <rdfs:subClassOf rdf:resource="http://rs.tdwg.org/ontology/Base#BaseThing"/>
      <rdfs:isDefinedBy rdf:resource="http://rs.tdwg.org/ontology/voc/Team"/>
   </owl:Class>
   
   
   <!-- awaiting final metadata strategy 
   <owl:DatatypeProperty rdf:ID="dcMemberTitle">
      <rdfs:label>Dublin Core Title</rdfs:label>
      <rdfs:comment> Dublin Core Metadata Title for this object. 
         This property should contain a string representation of the TeamMember as it might appear in printed publication.
         This property is represented in the TDWG Ontology as http://rs.tdwg.org/ontology/voc/Team#dcMemberTitle but it is good practise to use the Dublin Core equivalent
         http://purl.org/dc/elements/1.1/title in instance documents as it has the same meaning but it understandable to more clients. </rdfs:comment>
      <rdfs:domain rdf:resource="#TeamMember"/>
      <rdfs:range rdf:resource="http://www.w3.org/2001/XMLSchema#string"/>
      <owl:sameAs rdf:resource="http://purl.org/dc/elements/1.1/title"/>
      <rdfs:isDefinedBy rdf:resource="http://rs.tdwg.org/ontology/voc/Team"/>
   </owl:DatatypeProperty>
   -->


   <!-- TeamMember::member -->
   <owl:ObjectProperty rdf:ID="member">
      <rdfs:label>Member</rdfs:label>
      <rdfs:comment>The member who has this role and position.</rdfs:comment>
      <rdfs:domain rdf:resource="#TeamMember"/>
      <rdfs:range rdf:resource="http://rs.tdwg.org/ontology/voc/Person#Person"/>
      <rdfs:isDefinedBy rdf:resource="http://rs.tdwg.org/ontology/voc/Team"/>
   </owl:ObjectProperty>

   <!-- TeamMember::role -->
   <owl:DatatypeProperty rdf:ID="role">
      <rdfs:label>Role</rdfs:label>
      <rdfs:comment>The members role within the team e.g. Combination Author or Basionym Author.</rdfs:comment>
      <rdfs:domain rdf:resource="#TeamMember"/>
      <rdfs:range rdf:resource="http://www.w3.org/2001/XMLSchema#string"/>
      <rdfs:isDefinedBy rdf:resource="http://rs.tdwg.org/ontology/voc/Team"/>
   </owl:DatatypeProperty>

   <!-- TeamMember::index -->
   <owl:DatatypeProperty rdf:ID="index">
      <rdfs:label>index</rdfs:label>
      <rdfs:comment>The position of the person within the ordering of team members. The client might
         expect that ordering the members of team by the values of this property would place them in
         correct order. If more than one member has the same value then the behaviour is undefined.</rdfs:comment>
      <rdfs:domain rdf:resource="#TeamMember"/>
      <rdfs:range rdf:resource="http://www.w3.org/2001/XMLSchema#integer"/>
      <rdfs:isDefinedBy rdf:resource="http://rs.tdwg.org/ontology/voc/Team"/>
   </owl:DatatypeProperty>

</rdf:RDF>
