<?xml version="1.0" encoding="UTF-8"?>

<!-- $Author: RogerHyam $ -->
<rdf:RDF xmlns:rdf="http://www.w3.org/1999/02/22-rdf-syntax-ns#" xmlns:rdfs="http://www.w3.org/2000/01/rdf-schema#" xmlns:owl="http://www.w3.org/2002/07/owl#"
   xmlns:dc="http://purl.org/dc/elements/1.1/" xmlns:dcterms="http://purl.org/dc/terms/" xml:base="http://rs.tdwg.org/ontology/Base" xmlns="http://rs.tdwg.org/ontology/Base#">

   <owl:Ontology rdf:about="http://rs.tdwg.org/ontology/Base">
      <dc:creator>Robert Gales / Roger Hyam</dc:creator>
      <dcterms:issued>2006-05-26</dcterms:issued>
      <dcterms:modified>$Date: 2007-09-10 16:55:47 +0100 (Mon, 10 Sep 2007) $</dcterms:modified>
      <dc:title>TDWG Ontology - Base</dc:title>
      <dc:publisher>TDWG Biodiversity Information Standards</dc:publisher>
      <dc:description> The Base Ontology contains the highest level classes and attributes within the TDWG ontology which are typically not domain specific entities. </dc:description>

      <rdfs:comment rdf:parseType="Literal"> This ontology has been demonstrated to be valid RDF of the OWL-Lite subset by the following online tool: <a
            href="http://phoebus.cs.man.ac.uk:9999/OWL/Validator">Wonder Web OWL Ontology Validator</a>
      </rdfs:comment>

      <owl:versionInfo>0.3</owl:versionInfo>

   </owl:Ontology>

   <!-- BaseThing -->
   <owl:Class rdf:ID="BaseThing">
      <rdfs:label>Base Thing</rdfs:label>
      <rdfs:comment> The BaseThing represents the root object within the TDWG ontology. All classes within the ontology should be a direct or indirect subclass of it. At this time there are no
         properties that are necessary to define on this object as they are covered by global annotation properties. </rdfs:comment>
      <rdfs:isDefinedBy rdf:resource="http://rs.tdwg.org/ontology/Base"/>
   </owl:Class>

   <!-- Actor -->
   <owl:Class rdf:ID="Actor">
      <rdfs:label>Actor</rdfs:label>
      <rdfs:comment> The Base Actor represents any object that may perform an action. These may be people, organisations or software agents. Outside of the global properties that may be defined
         through Dublin Core or OWL Lite natively, no additional properties have been defined on this class. </rdfs:comment>
      <rdfs:subClassOf rdf:resource="#BaseThing"/>
      <rdfs:isDefinedBy rdf:resource="http://rs.tdwg.org/ontology/Base"/>
   </owl:Class>

   <!-- Space -->
   <owl:Class rdf:ID="Space">
      <rdfs:label>Space</rdfs:label>
      <rdfs:comment> The Base Space class represents a 2d or 3d geometry for describing a space. </rdfs:comment>
      <rdfs:subClassOf rdf:resource="#BaseThing"/>
      <rdfs:isDefinedBy rdf:resource="http://rs.tdwg.org/ontology/Base"/>
   </owl:Class>

   <!-- Name -->
   <owl:Class rdf:ID="Name">
      <rdfs:label>Name</rdfs:label>
      <rdfs:comment> The Base Name class represents the highest level base class for any representation of a name. </rdfs:comment>
      <rdfs:subClassOf rdf:resource="#BaseThing"/>
      <rdfs:isDefinedBy rdf:resource="http://rs.tdwg.org/ontology/Base"/>
   </owl:Class>

   <!-- DefinedTerm -->
   <owl:Class rdf:ID="DefinedTerm">
      <rdfs:label>Defined Term</rdfs:label>
      <rdfs:comment>The Base DefinedTerm represents a class for constructing controlled vocabularies of defined terminology. Known subclasses <a href="http://rs.tdwg.org/ontology/voc/TaxonRank#TaxonRank"
            >TaxonRankTerm</a> and <a href="http://rs.tdwg.org/ontology/voc/TDMTerm#TDMTerm">TDMTerm</a></rdfs:comment>
      <rdfs:subClassOf rdf:resource="#BaseThing"/>
      <rdfs:isDefinedBy rdf:resource="http://rs.tdwg.org/ontology/Base"/>
   </owl:Class>

   <!-- BaseDefinedTerm::definition -->
   <owl:DatatypeProperty rdf:ID="definition">
      <rdfs:label>Definition</rdfs:label>
      <rdfs:comment> A definition of a defined term. </rdfs:comment>
      <rdf:type rdf:resource="http://www.w3.org/2002/07/owl#DatatypeProperty"/>
      <rdfs:domain rdf:resource="#DefinedTerm"/>
      <rdfs:range rdf:resource="http://www.w3.org/2001/XMLSchema#string"/>
      <rdfs:isDefinedBy rdf:resource="http://rs.tdwg.org/ontology/Base"/>
   </owl:DatatypeProperty>

   <!-- BaseMediaObject -->
   <owl:Class rdf:ID="MediaObject">
      <rdfs:label>Media Object</rdfs:label>
      <rdfs:comment> The Base MediaObject represents a basic level of understanding for a multimedia object and may be extended to add additional properties. </rdfs:comment>
      <rdfs:subClassOf rdf:resource="#BaseThing"/>
      <rdfs:isDefinedBy rdf:resource="http://rs.tdwg.org/ontology/Base"/>
   </owl:Class>



</rdf:RDF>
