<?xml version="1.0" encoding="UTF-8"?>

<!-- $Author: RogerHyam $ -->
<rdf:RDF xmlns:rdf="http://www.w3.org/1999/02/22-rdf-syntax-ns#"
         xmlns:rdfs="http://www.w3.org/2000/01/rdf-schema#"
         xmlns:owl="http://www.w3.org/2002/07/owl#"
         xmlns:dc="http://purl.org/dc/elements/1.1/"
         xmlns:dcterms="http://purl.org/dc/terms/"
         xml:base="http://rs.tdwg.org/ontology/Core"
         xmlns:tcore="http://rs.tdwg.org/ontology/Core#"
         xmlns="http://rs.tdwg.org/ontology/Core#">

   <owl:Ontology rdf:about="http://rs.tdwg.org/ontology/Core">
      <dc:creator>Robert Gales / Roger Hyam</dc:creator>
      <dcterms:issued>2006-1-28</dcterms:issued>
      <dcterms:modified>2015-07-01</dcterms:modified>
      <dc:title>TDWG Ontology - Core</dc:title>
      <dc:publisher>Taxonomic Databases Working Group</dc:publisher>
      <dc:description>
         The Core Ontology represents extension to the Base Ontology describing high
         level general concepts that may be extended to represent Biology &amp; Biodiversity
         Informatics domain specific classes and properties.
      </dc:description>
      
      <dc:relation rdf:resource="http://rs.tdwg.org/ontology/Base"/>
      
      <rdfs:comment rdf:parseType="Literal"></rdfs:comment>
      
      <owl:versionInfo>0.4</owl:versionInfo>
      
      <owl:imports rdf:resource="http://rs.tdwg.org/ontology/Base"/>
      <owl:deprecated rdf:datatype="http://www.w3.org/2001/XMLSchema#boolean">true</owl:deprecated>
      <rdfs:comment>This ontology is no longer under development and is no longer recommended for use.  See https://github.com/tdwg/ontology for information about recommended replacements.</rdfs:comment>
      <rdfs:seeAlso rdf:resource="https://raw.githubusercontent.com/tdwg/ontology/master/replacements.rdf"/>
      
   </owl:Ontology>

   <!-- *********************************************************************************
   C L A S S E S
   ***********************************************************************************-->
   
   <!-- ContactInformation -->
   <owl:Class rdf:ID="ContactInformation">
      <rdfs:label>Contact Information</rdfs:label>
      <rdfs:comment>
         A class representing the base for which any contact information should be
         extended. Contact information should describe some manner in which a person or software
         agent may contact a person or organisation.
      </rdfs:comment>
      <rdfs:subClassOf rdf:resource="http://rs.tdwg.org/ontology/Base#BaseThing"/>
      <rdfs:isDefinedBy rdf:resource="http://rs.tdwg.org/ontology/Core"/>
   </owl:Class>
   
   <!-- Organisation -->
   <owl:Class rdf:ID="Organisation">
      <rdfs:label>Core Organisation</rdfs:label>
      <rdfs:comment rdf:parseType="Literal">
         An establishment, organization, or association, instituted for the promotion of some
         object, esp. one of public or general utility.
      </rdfs:comment>
      <rdfs:subClassOf rdf:resource="http://rs.tdwg.org/ontology/Base#Actor"/>
      <rdfs:isDefinedBy rdf:resource="http://rs.tdwg.org/ontology/Core"/>
   </owl:Class>
   
   <!-- Collection -->
   <owl:Class rdf:ID="Collection">
      <rdfs:label>Collection</rdfs:label>
      <rdfs:comment rdf:parseType="Literal">
         <p>
            A number of objects collected or gathered together, viewed as a whole, [...] of
            scientific specimens, objects of interest, works of art, etc.[1]
         </p>
         <p>1. Oxford English Dictionary</p>
      </rdfs:comment>
      <rdfs:subClassOf rdf:resource="http://rs.tdwg.org/ontology/Base#BaseThing"/>
      <rdfs:isDefinedBy rdf:resource="http://rs.tdwg.org/ontology/Core"/>
   </owl:Class>

   <!-- Description -->
   <owl:Class rdf:ID="Description">
      <rdfs:label>Description</rdfs:label>
      <rdfs:comment rdf:parseType="Literal">
         <p>
            A Statement which describes, sets forth or portrays; a graphic or detailed account of a
            thing.[1]
         </p>
         <p>1. Oxford English Dictionary</p>
      </rdfs:comment>
      <rdfs:subClassOf rdf:resource="http://rs.tdwg.org/ontology/Base#BaseThing"/>
      <rdfs:isDefinedBy rdf:resource="http://rs.tdwg.org/ontology/Core"/>
   </owl:Class>

   <!-- Geolocalisation -->
   <owl:Class rdf:ID="Geolocalisation">
      <rdfs:label>Core Geolocalisation</rdfs:label>
      <rdfs:comment>
         An object that represents the artifact of a geolocalisation event, where a
         geolocalisation event is the identification of a specific place from only textual
         representations of the locality.
      </rdfs:comment>
      <rdfs:subClassOf rdf:resource="http://rs.tdwg.org/ontology/Base#BaseThing"/>
      <rdfs:isDefinedBy rdf:resource="http://rs.tdwg.org/ontology/Core"/>
   </owl:Class>

   <!-- Person -->
   <owl:Class rdf:ID="Person">
      <rdfs:label>Person</rdfs:label>
      <rdfs:comment rdf:parseType="Literal">
         <p>An individual human being.[1]</p>
         <p>1. Oxford English Dictionary</p>
      </rdfs:comment>
      <rdfs:subClassOf rdf:resource="http://rs.tdwg.org/ontology/Base#BaseActor"/>
      <rdfs:isDefinedBy rdf:resource="http://rs.tdwg.org/ontology/Core"/>
   </owl:Class>

   <!-- Place -->
   <owl:Class rdf:ID="Place">
      <rdfs:label>Place</rdfs:label>
      <rdfs:comment rdf:parseType="Literal">
         <p>
            A particular part of space of defined or undefined extent but of definite situation.
            [1]
         </p>
         <p>1. Oxford English Dictionary</p>
      </rdfs:comment>
      <rdfs:subClassOf rdf:resource="http://rs.tdwg.org/ontology/Base#BaseThing"/>
      <rdfs:isDefinedBy rdf:resource="http://rs.tdwg.org/ontology/Core"/>
   </owl:Class>

   <!-- PublicationCitation -->
   <owl:Class rdf:ID="PublicationCitation">
      <rdfs:label>Publication Citation</rdfs:label>
      <rdfs:comment rdf:parseType="Literal">
         <p>
            A citation or bibliographic citation is a reference to a book, article, web page or
            other published item, with sufficient details to uniquely identify the item. [1]
         </p>
         <p>
            1. <a href="http://en.wikipedia.org/wiki/Citation">http://en.wikipedia.org/wiki/Citation</a>
         </p>
      </rdfs:comment>
      <rdfs:subClassOf rdf:resource="http://rs.tdwg.org/ontology/Base#BaseThing"/>
      <rdfs:isDefinedBy rdf:resource="http://rs.tdwg.org/ontology/Core"/>
   </owl:Class>

   <!-- Specimen -->
   <owl:Class rdf:ID="Specimen">
      <rdfs:label>Specimen</rdfs:label>
      <rdfs:comment rdf:parseType="Literal">
         <p>
            An animal, plant, or mineral, a part or portion of some substance or organism, etc.,
            serving as an example of the thing in question for purposes of investigation or
            scientific study.[1]
         </p>
         <p>1. Oxford English Dictionary</p>
      </rdfs:comment>
      <rdfs:subClassOf rdf:resource="http://rs.tdwg.org/ontology/Base#BaseThing"/>
      <rdfs:isDefinedBy rdf:resource="http://rs.tdwg.org/ontology/Core"/>
   </owl:Class>

   <!-- Concept -->
   <owl:Class rdf:ID="Concept">
      <rdfs:label>Concept</rdfs:label>
      <rdfs:comment>
         an abstract or general idea inferred or derived from specific instances
      </rdfs:comment>
      <rdfs:subClassOf rdf:resource="http://rs.tdwg.org/ontology/Base#BaseThing"/>
      <rdfs:isDefinedBy rdf:resource="http://rs.tdwg.org/ontology/Core"/>
   </owl:Class>

   <!-- Identification -->
   <owl:Class rdf:ID="Identification">
      <rdfs:label>Identification</rdfs:label>
      <rdfs:comment>
         The identification of a specimen to a specific concept.
      </rdfs:comment>
      <rdfs:subClassOf rdf:resource="http://rs.tdwg.org/ontology/Base#BaseThing"/>
      <rdfs:isDefinedBy rdf:resource="http://rs.tdwg.org/ontology/Core"/>
   </owl:Class>
   
   <!-- Team -->
   <owl:Class rdf:ID="Team">
      <rdfs:label>Team</rdfs:label>
      <rdfs:comment rdf:parseType="Literal">
         <p>a group of people (CorePerson) linked in a common purpose[1]</p>
         <p>1. en.wikipedia.org</p>
      </rdfs:comment>
      <rdfs:subClassOf rdf:resource="http://rs.tdwg.org/ontology/Base#Actor"/>
      <rdfs:isDefinedBy rdf:resource="http://rs.tdwg.org/ontology/Core"/>
   </owl:Class>

   <!-- Observation -->
   <owl:Class rdf:ID="Observation">
      <rdfs:label>Observation</rdfs:label>
      <rdfs:comment>
         A record of the observation of some concept at a particular location and time.
      </rdfs:comment>
      <rdfs:subClassOf rdf:resource="http://rs.tdwg.org/ontology/Base#BaseThing"/>
      <rdfs:isDefinedBy rdf:resource="http://rs.tdwg.org/ontology/Core"/>
   </owl:Class>

   <!-- Gathering -->
   <owl:Class rdf:ID="Gathering">
      <rdfs:label>Gathering</rdfs:label>
      <rdfs:comment>
         A record of the event of gathering specimens at a particular location over a
         specific time period.
      </rdfs:comment>
      <rdfs:subClassOf rdf:resource="http://rs.tdwg.org/ontology/Base#BaseThing"/>
      <rdfs:isDefinedBy rdf:resource="http://rs.tdwg.org/ontology/Core"/>
   </owl:Class>

</rdf:RDF>
